feat: SSReflectを使用して書き換え

src/Michio Suzuki (1982) Group Theory I/main.v
@@ -1,71 +1,66 @@
 (* Suzuki, Michio - Group Theory. I *)
+From mathcomp
+  Require Import ssreflect.
+Require Import Coq.Sets.Ensembles.
 
 (* Definition 1.1. *)
-Structure Group : Type := mkGroup
+Structure Group (T : Type) : Type := mkGroup
 {
-  G :> Set;
-  non_emp : exists (x : G), True;
-  mul : G -> G -> G;
-  mul_assoc : forall a b c, mul (mul a b) c = mul a (mul b c);
-  inv_mul : forall a b, exists x, mul a x = b;
-  mul_inv : forall a b, exists y, mul y a = b;
+  G :> Ensemble T;
+  non_emp : exists x : T, In T G x;
+  mul : T -> T -> T;
+  mul_closed : forall a b : T, In T G a -> In T G b -> In T G (mul a b);
+  mul_assoc : forall a b c : T, mul (mul a b) c = mul a (mul b c);
+  inv_mul : forall a b : T, exists x, mul a x = b;
+  mul_inv : forall a b : T, exists y, mul y a = b;
 }.
 
-Arguments mul {g} _ _.
-
 (* Definition 1.3. *)
-Definition is_identity (G : Group) (e : G) :=
-  forall (g : G), mul g e = g /\ mul e g = g.
+Definition is_identity (T : Type) (G : Group T) (e : T) :=
+  forall g : T, mul T G g e = g /\ mul T G e g = g.
 
 (* Theorem 1.2.(ii)' *)
-Theorem one_exists_unique (G : Group) :
-  exists! (one : G), is_identity G one.
+Theorem one_exists_unique (T : Type) (G : Group T) :
+  exists! one : T, is_identity T G one.
 Proof.
-  destruct (non_emp G) as [a h0].
-  destruct (inv_mul G a a) as [e h1].
-  destruct (mul_inv G a a) as [e' h2].
+  destruct (non_emp T G) as [a HaInG].
+  destruct (inv_mul T G a a) as [e HaeEqa].
+  destruct (mul_inv T G a a) as [e' He'aEqa].
   exists e.
+  
+  assert (forall g : T, mul T G g e = g) as He_r_id.
+  + move=> g.
+    destruct (inv_mul T G a g) as [u HauEqg].
+    destruct (mul_inv T G a g) as [v HvaEqg].
+    rewrite -HvaEqg.
+    rewrite mul_assoc.
+    rewrite HaeEqa.
+    by [].
 
-  assert (forall g : G, mul g e = g) as h3.
-    intro g.
-      destruct (inv_mul G a g) as [u h3_1].
-      destruct (mul_inv G a g) as [v h3_2].
+  assert (forall g : T, mul T G e' g = g) as He'_l_id.
+  + move=> g.
+    destruct (inv_mul T G a g) as [u HauEqg].
+    destruct (mul_inv T G a g) as [v HvaEqg].
+    rewrite -HauEqg.
+    rewrite -mul_assoc.
+    rewrite He'aEqa.
+    by [].
 
-      rewrite <- h3_2.
-      rewrite -> mul_assoc.
-      rewrite -> h1.
-      reflexivity.
-
-  assert (forall g : G, mul e' g = g) as h4.
-    intro g.
-      destruct (inv_mul G a g) as [u h4_1].
-      destruct (mul_inv G a g) as [v h4_2].
-
-      rewrite <- h4_1.
-      rewrite <- mul_assoc.
-      rewrite -> h2.
-      reflexivity.
-
-  assert (e = e') as h5.
-    rewrite <- (h3 e').
-    rewrite -> (h4 e).
-    reflexivity.
+  assert (e = e') as HeEqe'.
+  + rewrite -(He_r_id e').
+    rewrite (He'_l_id e).
+    by [].
 
   split.
-
-  intro g.
-  split.
-    apply (h3 g).
-
-    rewrite -> h5.
-    rewrite -> (h4 g).
-    reflexivity.
-
-  intro g.
-  intro h6.
-
-  destruct (h6 e) as [h7 h8].
-  rewrite <- (h3 g).
-  rewrite -> h8.
-  reflexivity.
+  + move=> g.
+    split.
+    + apply (He_r_id g).
+    + rewrite HeEqe'.
+      rewrite (He'_l_id g).
+      by [].
+  + move=> g Hg_id.
+    destruct (Hg_id e) as [HegEqe HgeEqe].
+    rewrite -(He_r_id g).
+    rewrite HgeEqe.
+    by [].
 Qed.
